kalloc/Verif_clients.v
@@ -406,9 +406,50 @@ Definition kfree_loop_spec :=
                 KF_globals gv sh (added_elem++ls) xx head
             ).
 
-Definition KFGprog_clients: funspecs := KFGprog ++ [kalloc_write_pipe_spec; kfree_kalloc_spec; kalloc_write_42_spec; kalloc_write_42_kfree_spec].
+Definition kfree_loop_kalloc_spec := 
+    DECLARE _kfree_loop_kalloc
+    WITH sh : share, pa1:val, original_freelist_pointer:val, xx:Z, gv:globals, ls : list val, n:Z
+    PRE [ tptr tvoid, tint ]
+        PROP(
+            isptr pa1 /\
+            Int.min_signed <= Int.signed (Int.repr n) + Int.signed (Int.repr 1) <= Int.max_signed /\
+            0 <= n <= Int.max_signed
+        ) 
+        PARAMS (pa1; Vint (Int.repr n)) GLOBALS(gv)
+        SEP (
+            kalloc_tokens Tok_APD sh (Z.to_nat n)%nat pa1 PGSIZE t_run *
+            KF_globals gv sh ls xx original_freelist_pointer
+        )
+    POST [ tptr tvoid ]
+        EX head, EX added_elem, (* TODO: fix top and next is the same?? *)
+        PROP( 
+            (* before alloc *)
+            added_elem = (pointers_with_original_head (Z.to_nat n) (pa1) PGSIZE original_freelist_pointer) /\
+            head = (hd nullval ((pointers_with_original_head (Z.to_nat n+1) (pa1) PGSIZE original_freelist_pointer)++ls))
+            )
+            RETURN (head) (* we return the head like in the pop function*)
+            SEP 
+            (
+            let n_eq_0_case :=
+                if eq_dec original_freelist_pointer nullval then
+                emp * KF_globals gv sh ls xx original_freelist_pointer
+            else
+                EX next, EX ls',
+                    !! (next :: ls' = ls) &&
+                    KF_globals gv sh ls' xx next *
+                    kalloc_token' KF_APD sh (sizeof t_run) original_freelist_pointer
+            in
+            let n_gt_0_case :=
+                KF_globals gv sh ((tl added_elem)++ls) xx (hd nullval added_elem) *
+                kalloc_token' KF_APD sh (sizeof t_run) head
+            in
+            if (Z.ltb 0 n) then
+                n_gt_0_case
+            else 
+                n_eq_0_case
+                ).
 
-
+Definition KFGprog_clients: funspecs := KFGprog ++ [kalloc_write_pipe_spec; kfree_kalloc_spec; kalloc_write_42_spec; kalloc_write_42_kfree_spec; kfree_loop_spec].
 
 Lemma body_kalloc_write_pipe: semax_body KFVprog KFGprog f_kalloc_write_pipe kalloc_write_pipe_spec.
 Proof.
@@ -916,4 +957,48 @@ Intros. forward. (*forward. unfold abb iate in POSTCONDITION.*)
     rewrite H0021.  rewrite sub_add_offset_n; auto; try rep_lia.
     replace (Z.of_nat (n0 - 0)) with (i -1); try rep_lia. auto.
     unfold PGSIZE; rep_lia.
+Qed.
+
+
+Lemma body_kfree_loop_kalloc: semax_body KFVprog KFGprog_clients f_kfree_loop_kalloc kfree_loop_kalloc_spec.
+Proof.
+start_function.
+forward_call (sh, pa1:val, original_freelist_pointer:val, xx:Z, gv:globals, ls : list val, n:Z).
+- destruct H as [H1 [H2 H3]]; auto.
+- Intros vret. 
+forward_call (kalloc_spec_sub KF_APD t_run) (gv, sh , snd vret ++ ls, xx,  fst vret ); (* kalloc *)
+destruct H as [H11 [H12 H13]]; auto.
+    + unfold KF_globals. entailer!.
+    + if_tac; auto_contradict.
+        * forward. destruct (Z.to_nat n) eqn:en.
+            -- assert (n = 0); try rep_lia. rewrite H3. Exists (fst vret) (snd vret).
+                    entailer.
+                    if_tac_auto_contradict;
+                    destruct (0 <? 0) eqn:efalse; try rep_lia.
+                ++simpl in H0. rewrite H0. simpl in H1. rewrite H1. unfold KF_globals. rewrite app_nil_l. entailer!.
+                ++simpl in H1. rewrite <- H1 in H3. rewrite H in H3; auto_contradict.
+            -- rewrite <- add_to_pointers_with_head in H1; auto; try rep_lia. simpl in H1.
+            assert (isptr (offset_val (Z.of_nat (n0 - 0) * PGSIZE) pa1)). { apply isptr_offset_val'. auto. }
+            rewrite <- H1 in H3. rewrite H in H3; auto_contradict.
+        * forward. destruct (Z.to_nat n) eqn:en.
+            -- Exists (fst vret) (snd vret).
+                assert (n = 0); try rep_lia. rewrite H4.
+                if_tac_auto_contradict;
+                destruct (0 <? 0) eqn:efalse; try rep_lia.
+                ++ unfold KF_globals. entailer!.
+                ++ destruct ls eqn:els.
+                    **  simpl in H0. rewrite H0 in H3. inversion H3.
+                    ** simpl in H1. simpl in H0. Exists (fst ab) (snd ab). unfold KF_globals. rewrite H1.
+                    entailer!. rewrite H0 in H3. rewrite app_nil_l in H3. auto.
+                    unfold my_kalloc_token. entailer!.
+            -- Exists (fst vret) (snd vret).
+                entailer.
+                destruct (0 <? n) eqn:etrue; try rep_lia.
+                unfold KF_globals. unfold my_kalloc_token. entailer!.
+                destruct (snd vret).
+                ++ replace (S n0) with (n0 + 1)%nat in H0; try rep_lia. 
+                destruct n0 eqn:en0.
+                ** simpl in H0. inversion H0.
+                ** rewrite  <- add_to_pointers_with_head in H0; auto; try rep_lia. inversion H0.
+                ++ simpl. rewrite <- app_comm_cons in H3. inversion H3. entailer.
 Qed.
